VerusLean/VLIR/Parser.lean
@@ -6,12 +6,17 @@ import Lean
 namespace VerusLean
 
 open Lean
+open VName
 
 /-- A map for variables. Alias for `Std.HashMap Ident Typ`. -/
 abbrev VarMap := Std.HashMap Ident Typ
 
 /-- A map for functions. Alias for `Std.HashMap Ident SpecFn`. -/
 abbrev FnMap := Std.HashMap Ident SpecFn
+
+abbrev DtMap := Std.HashMap Ident Struct
+
+abbrev DeclMap := Std.HashMap Ident Decl
 
 /--
   The parsing monad for Verus JSONs,
@@ -29,8 +34,8 @@ structure ParserState where
   freeVars : VarMap := {}
   -- Acts like a stack?
   boundVars : List Ident := []
-  fns : FnMap := {}
-deriving Inhabited
+  decls : DeclMap := {}
+deriving Inhabited, Repr
 
 abbrev VParser := EStateM String ParserState
 
@@ -87,11 +92,11 @@ def withBoundVars (vars : List Ident) (fn : VParser α) : VParser α := do
   popBoundVars vars.length
   return a
 
-def addSpecFn (fn : SpecFn) : VParser Unit :=
-  modify fun st => { st with fns := st.fns.insert fn.name fn }
+def addDecl (d : Decl) : VParser Unit :=
+  modify fun st => { st with decls := st.decls.insert (name d) d }
 
-def setFns (fns : FnMap) : VParser Unit :=
-  modify fun st => { st with fns := fns }
+def getDecl? (i : Ident) : VParser (Option Decl) :=
+  do let st ← get; return st.decls.get? i
 
 def coeWithState : Except String α → VParser α
   | .ok a => (fun s => Result.ok a s)
@@ -109,14 +114,31 @@ end VParser
 
 open VParser
 
-def Typ.fromJson? (j : Json) : ExStr Typ := do
+variable {m : Type → Type} [Monad m] [MonadExceptOf String m]
+
+def xJsonFromSpanned (j : Json) : m Json :=
+  j.getObjValM "x"
+
+def widthFromJson (j : Json) : m Nat := do
+  j.getNatUnderKeyM "Width"
+
+-- TODO: This probably needs to return a namespace (list?), rather than a single ident
+def pathedNameFromJson (j : Json) (pathKey : String := "path") : m Ident := do
+  let pathed ← j.getObjValByPathM [pathKey, "segments"]
+  Json.getStrM <| ← Json.getArrValM pathed 0
+
+def pathedNameFromNameJson (j : Json) (pathKey : String := "path") : m Ident := do
+  let nameObj ← j.getObjValM "name"
+  pathedNameFromJson nameObj pathKey
+
+def Typ.fromJson (j : Json) : m Typ := do
   match j.getStr? with
   | .ok "Bool" => return .Bool
   | .ok _ => throw "unsupported primitive type"
   | .error _ =>
-    match ← j["Primitive", "Int", "ConstInt", "Array"] with
+    match ← j["Primitive", "Int", "ConstInt", "Array", "Datatype"] with
     | ("Primitive", obj) =>
-      let t ← obj.getArr?
+      let t ← obj.getArrM
       match t.get? 0 with
       | some "Array" => throw "unsupported primitive type Array"
       -- .ok (Typ.Array Typ.Int)
@@ -126,8 +148,8 @@ def Typ.fromJson? (j : Json) : ExStr Typ := do
     | ("Int", obj) =>
       -- First, we check if the the underlying string is "Int" for mathematical integers
       match obj.getStr? with
-      | .ok "Int" => .ok Typ.Int
-      | .ok "Nat" => .ok Typ.Nat
+      | .ok "Int" => return .Int
+      | .ok "Nat" => return .Nat
       | .ok _ => throw s!"unsupported Int object string: {obj}"
       | .error _ =>
         -- Now check if it is a fixed-width integer
@@ -135,13 +157,20 @@ def Typ.fromJson? (j : Json) : ExStr Typ := do
         | .error _ => throw s!"unsupported Int object: {obj}"
         | .ok ("U", obj) =>
           match obj.getNat? with
-          | .ok width => .ok (Typ.UInt width)
+          | .ok width => return Typ.UInt width
           | .error e => throw s!"[Typ.fromJson?]: {e}"
         | .ok ("I", obj) =>
           match obj.getNat? with
-          | .ok width => .ok (Typ.SInt width)
+          | .ok width => return Typ.SInt width
           | .error e => throw s!"[Typ.fromJson?]: {e}"
         | .ok _ => throw s!"unsupported Int object: {obj}"
+
+    | ("Datatype", obj) =>
+      let ⟨arr, _⟩ ← obj.getArrWithSizeGeM 3
+      let name ← pathedNameFromJson arr[0] "Path"
+      -- TODO: Ignoring parameters to the type for now
+      let params := []
+      return .Struct name params
 
     | _ => throw "unsupported primitive type"
 
@@ -151,66 +180,55 @@ def Typ.fromJson? (j : Json) : ExStr Typ := do
   Also adds the type annotation for the span to the state.
   This annotation should be added to the state's `HashMap` when encountering a `Var`.
 -/
-def fromJsonSpanned? {α : Type} (j : Json) (fj : Json → VParser α) : VParser α := do
-  let typ ← Typ.fromJson? <| ← j.getObjVal? "typ"
+def fromJsonSpanned {α : Type} (j : Json) (fj : Json → VParser α) : VParser α := do
+  let typ ← Typ.fromJson <| ← j.getObjVal? "typ"
   let x ← j.getObjVal? "x"
   setTyp typ
   fj x
 
-def xJsonFromSpanned? (j : Json) : ExStr Json :=
-  j.getObjVal? "x"
-
-def widthFromJson? (j : Json) : ExStr Nat := do
-  j.getNatUnderKey? "Width"
-
--- TODO: This probably needs to return a namespace (list?), rather than a single ident
-def pathedNameFromJson? (j : Json) : ExStr Ident := do
-  let pathed ← j.getObjValByPath ["path", "segments"]
-  Json.getStr? <| ← Json.getArrVal? pathed 0
-
 --------------------------------------------------------------------------------
 
-def Mode.fromJson? (j : Json) : ExStr Mode := do
-  match ← j.getStr? with
+def Mode.fromJson (j : Json) : m Mode := do
+  match ← j.getStrM with
   | "Spec"  => return .Spec
   | "Proof" => return .Proof
   | "Exec"  => return .Exec
   | str => throw s!"[Mode.fromJson?]: Expected one of \{ Spec, Proof, Exec }, got {str}"
 
-def Const.fromJson? (j : Json) : ExStr Const := do
+def Const.fromJson (j : Json) : m Const := do
   match ← j["Bool", "Int", "StrSlice", "Char"] with
-  | ("Bool", v) => return Const.Bool <| ← v.getBool?
+  | ("Bool", v) => return Const.Bool <| ← v.getBoolM
   | ("Int", v) =>
     -- Ints are serialized as an array, with the first element the sign enum
     -- and the second value is the data, an array of u64s.
-    let ⟨arr, _⟩ ← v.getArrWithSizeGe? 2
+    let ⟨arr, _⟩ ← v.getArrWithSizeGeM 2
     let s := arr[0]
     let n := arr[1]
-    match ← s.getNat? with
+    match ← s.getNatM with
     | 0 =>
       -- no sign
       -- CZ: according to bigint.rs, 0 is minus, 1 is no sign, 2 is plus?
-      .ok (Const.Int 0)
+      return Const.Int 0
     | 1 =>
       -- positive number
       -- TODO: Need some computation for the big int
       -- For now, take the first entry and move on
-      let nArr ← n.getArr?
+      let nArr ← n.getArrM
       let n := nArr.getD 0 (Json.num <| JsonNumber.fromNat 0)
-      return Const.Int <| Int.ofNat <| ← n.getNat?
+      return Const.Int <| Int.ofNat <| ← n.getNatM
     | 2 =>
       -- negative number
       -- TODO: Need some computation for the big int
       -- For now, take the first entry and move on
-      let nArr ← n.getArr?
+      let nArr ← n.getArrM
       let n := nArr.getD 0 (Json.num <| JsonNumber.fromNat 0)
-      return Const.Int <| -(Int.ofNat <| ← n.getNat?)
+      return Const.Int <| -(Int.ofNat <| ← n.getNatM)
     | _ => throw "[Const.fromJson?]: Expected an Int sign of 0, 1, or 2"
   | ("StrSlice", _) => throw "not yet implemented"
   | ("Char", _) => throw "not yet implemented"
   | _ => throw "[Const.fromJson?]: Unexpected match"
 
-def Bitwise.fromJson? (j : Json) : ExStr BitwiseOp :=
+def Bitwise.fromJson (j : Json) : m BitwiseOp :=
   match j.getStr? with
   | .ok "BitXor" => return .BitXor
   | .ok "BitAnd" => return .BitAnd
@@ -221,34 +239,34 @@ def Bitwise.fromJson? (j : Json) : ExStr BitwiseOp :=
     -- They are Json objects that store the width (and sign extension)
     match ← j["Shr", "Shl"] with
     | ("Shr", obj) => do
-      let width ← widthFromJson? obj
+      let width ← widthFromJson obj
       return .Shr width
 
     | ("Shl", obj) =>
-      let ⟨arr, _⟩ ← obj.getArrWithSizeGe? 2
-      let width ← widthFromJson? arr[0]
-      return .Shl width (← arr[1].getBool?)
+      let ⟨arr, _⟩ ← obj.getArrWithSizeGeM 2
+      let width ← widthFromJson arr[0]
+      return .Shl width (← arr[1].getBoolM)
 
     | _ => throw s!"[Bitwise.fromJson?]: Expected one of \{ Shr, Shl }, got {j}"
 
-def ArithOp.fromJson? (j : Json) : ExStr ArithOp := do
-  match ← j.getStr? with
+def ArithOp.fromJson (j : Json) : m ArithOp := do
+  match ← j.getStrM with
   | "Add"          => return .Add
   | "Sub"          => return .Sub
   | "Mul"          => return .Mul
   | "EuclideanDiv" => return .EuclideanDiv
   | "EuclideanMod" => return .EuclideanMod
-  | s => throw s!"[ArithOp.fromJson?]: Expected one of Add, Sub, Mul, Div, Mod, got {s}"
+  | s => throw s!"[ArithOp.fromJson?]: Expected one of \{ Add, Sub, Mul, Div, Mod }, got {s}"
 
-def InequalityOp.fromJson? (j : Json) : ExStr InequalityOp := do
-  match ← j.getStr? with
+def InequalityOp.fromJson (j : Json) : m InequalityOp := do
+  match ← j.getStrM with
   | "Le" => return .Le
   | "Ge" => return .Ge
   | "Lt" => return .Lt
   | "Gt" => return .Gt
   | s => throw s!"[InequalityOp.fromJson?]: Expected one of \{ Le, Ge, Lt, Gt }, got {s}"
 
-def UnaryOp.fromJson? (j : Json) : ExStr UnaryOp := do
+def UnaryOp.fromJson (j : Json) : m UnaryOp := do
   match j.getStr? with
   | .ok "Not"    => return .Not
   | .ok "BitNot" => throw "not yet implemented"
@@ -258,12 +276,37 @@ def UnaryOp.fromJson? (j : Json) : ExStr UnaryOp := do
     -- Try seeing if "BitNot" has a width
     match ← j["BitNot", "Trigger"] with
     | ("BitNot", obj) =>
-      let width ← widthFromJson? obj
+      let width ← widthFromJson obj
       return .BitNot width
     | ("Trigger", _) => return .Trigger
     | _ => throw s!"[UnaryOp.fromJson?]: Expected one of \{ BitNot, Trigger }, got {j}"
 
-def BinaryOp.fromJson? (j : Json) : ExStr BinaryOp :=
+/--
+  Parses a unary operation under the "UnaryOpr" key.
+
+  Verus divides unary operations into simple and complex operations.
+  Simple ones are generally logical or bitwise operations,
+  and are parsed by `UnaryOp.fromJson?`.
+  This function parses the complicated ones: projection, etc.
+
+  -- TODO: Combine into `UnaryOp.fromJson?`?
+  -- TODO: Require the parser state to refer to data types?
+-/
+def UnaryOp.oprFromJson (j : Json) : m UnaryOp := do
+  match ← j["Field", "IsVariant"] with
+  | ("Field", obj) =>
+    -- TODO: Skipping data type
+    let variant ← obj.getStrUnderKeyM "variant"
+    let field ← obj.getStrUnderKeyM "field"
+    return .Proj variant field
+  | ("IsVariant", obj) =>
+    -- TODO: Skipping data type
+    let variant ← obj.getStrUnderKeyM "variant"
+    return .IsVariant variant "hello"
+  | _ =>
+    return .Trigger
+
+def BinaryOp.fromJson (j : Json) : m BinaryOp :=
   -- Most are single strings, but Eq has a mode attached, etc.
   match j.getStr? with
   | .ok "And"     => return .And
@@ -275,109 +318,145 @@ def BinaryOp.fromJson? (j : Json) : ExStr BinaryOp :=
   | .error _ => do
     -- Try one of the object ops instead
     match ← j["Eq", "Inequality", "Bitwise", "Arith"] with
-    | ("Eq", obj)         => return .Eq (← Mode.fromJson? obj)
-    | ("Inequality", obj) => return .Inequality (← InequalityOp.fromJson? obj)
+    | ("Eq", obj)         => return .Eq (← Mode.fromJson obj)
+    | ("Inequality", obj) => return .Inequality (← InequalityOp.fromJson obj)
     | ("Bitwise", obj) =>
       -- Object under "Bitwise" should be a two-element array with an op and a mode
-      let ⟨arr, _⟩ ← obj.getArrWithSizeGe? 2
-      let op ← Bitwise.fromJson? arr[0]
-      let mode ← Mode.fromJson? arr[1]
+      let ⟨arr, _⟩ ← obj.getArrWithSizeGeM 2
+      let op ← Bitwise.fromJson arr[0]
+      let mode ← Mode.fromJson arr[1]
       return .Bitwise op mode
     | ("Arith", obj) =>
       -- Object under "Arith" should be a two-element array with an op and a mode
-      let ⟨arr, _⟩ ← obj.getArrWithSizeGe? 2
-      let op ← ArithOp.fromJson? arr[0]
-      let mode ← Mode.fromJson? arr[1]
+      let ⟨arr, _⟩ ← obj.getArrWithSizeGeM 2
+      let op ← ArithOp.fromJson arr[0]
+      let mode ← Mode.fromJson arr[1]
       return .Arith op mode
     | _ => throw s!"[BinaryOp.fromJson?]: Expected one of \{ And, Or, Xor, Implies, Eq }, got something else: {j}"
 
-def Quant.fromJson? (j : Json) : ExStr Quant := do
-  match ← j.getObjVal? "quant" with
+def Quant.fromJson (j : Json) : m Quant := do
+  match ← j.getObjValM "quant" with
   | "Forall" => return .Forall
   | "Exists" => return .Exists
   | s => throw s!"[Quant.fromJson?]: Expected one of \{ Forall, Exists }, got {s}"
 
-def CallFun.fromJson? (j : Json) : ExStr CallFun := do
-  let obj ← j.getObjVal? "Fun"
-  let ⟨arr, _⟩ ← obj.getArrWithSizeGe? 1
-  return .Fun <| ← pathedNameFromJson? arr[0]
+def CallFun.fromJson (j : Json) : m CallFun := do
+  let ⟨arr, _⟩ ← j.getArrUnderKeyWithSizeGeM "Fun" 1
+  return .Fun <| ← pathedNameFromJson arr[0]
 
-def VarBinder.fromJson? (j : Json) : ExStr (VarBinder Typ) := do
-  let obj ← j.getObjVal? "name"
-  let ⟨arr, _⟩ ← obj.getArrWithSizeGe? 1
-  let name ← arr[0].getStr?
-  let typ ← Typ.fromJson? <| ← j.getObjVal? "typ"
-  return VarBinder.mk name typ
+def VarBinder.fromJson (j : Json) (key : String := "typ") : m (Ident × Typ) := do
+  let ⟨arr, _⟩ ← j.getArrUnderKeyWithSizeGeM "name" 1
+  let name ← arr[0].getStrM
+  let typ ← Typ.fromJson <| ← j.getObjValM key
+  return (name, typ)
 
-def VarBinder.fromJsonForBind? (j : Json) : ExStr (VarBinder Typ) := do
-  dbg_trace s!"Getting varbinder from {j}"
-  let obj ← j.getObjVal? "name"
-  let ⟨arr, _⟩ ← obj.getArrWithSizeGe? 1
-  let (name : String) ← arr[0].getStr?
-  let typ ← Typ.fromJson? <| ← j.getObjVal? "a"
-  return VarBinder.mk name typ
+def VarBinder.typBindersFromJson (j : Json) : m (List (Ident × Typ)) := do
+  let (arr : _root_.Array Json) ← j.getArrM
+  arr.toList.mapM (VarBinder.fromJson · "a")
 
-def VarBinder.typBindersFromJson? (j : Json) : ExStr (List (VarBinder Typ)) := do
-  let (arr : _root_.Array Json) ← j.getArr?
-  arr.toList.mapM VarBinder.fromJsonForBind?
 
 mutual /- {Bind, Exp}.fromJson? -/
 
-partial def Bind.fromJson? (j : Json) : VParser Bind := do
-  let obj : Json ← xJsonFromSpanned? j
+partial def Bind.fromJson (j : Json) : VParser Bind := do
+  let obj : Json ← xJsonFromSpanned j
   match ← obj.getFirstVal ["Quant"] with
   | ("Quant", (q : Json)) =>
-    let ⟨arr, _⟩ ← coeWithState <| q.getArrWithSizeGe? 4
-    let q ← Quant.fromJson? arr[0]
-    let binders ← VarBinder.typBindersFromJson? arr[1]
+    let ⟨arr, _⟩ ← q.getArrWithSizeGeM 4
+    let q ← Quant.fromJson arr[0]
+    let binders ← VarBinder.typBindersFromJson arr[1]
     return .Quant q binders
   | _ => throw "unexpected"
 
-partial def Exp.fromJson? (j : Json) : VParser Exp := do
+partial def Exp.fromJson (j : Json) : VParser Exp := do
   -- Expect that exactly one of the enumerated options will be true
-  match ← j["Const", "Var", "Unary", "Binary", "If", "Bind", "Call"] with
+  match ← j["Const", "Var", "Ctor", "Unary", "UnaryOpr", "Binary", "If", "Bind", "Call"] with
   | ("Const", obj) => do
-    return Exp.Const <| ← Const.fromJson? obj
+    return Exp.Const <| ← Const.fromJson obj
+
   | ("Var", obj) =>
     -- Verus gives us an array, where the first element is the identifier
-    let (i : Json) ← obj.getArrVal? 0
-    let (ident : Ident) ← i.getStr?
+    let i ← obj.getArrValM 0
+    let ident ← i.getStr?
     addFreeVarIfNotBound ident
     return .Var ident
+
+  | ("Ctor", obj) =>
+    let ⟨arr, _⟩ ← obj.getArrWithSizeGeM 3
+
+    let pathedName ← pathedNameFromJson arr[0] "Path"
+
+    /- TODO: This parsing code doesn't take into account more complicated
+      namespace pathing in Rust. We are assuming that all paths/variants
+      are contained in the same file. To be fixed later.  -/
+    let dt ← arr[1].getStrM
+
+    -- According to Verus, the order of the fields within a `Ctor` node
+    -- is unspecified, so parsing should not rely on field order.
+    let fields ← arr[2].getArrM
+
+    -- For each field, parse a field name and its expression
+    let parsedFields ← fields.mapM (fun fObj => do
+      let name ← Json.getStrUnderKeyM fObj "name"
+      -- The expression lies under two `Spanned` objects
+      -- TODO: Might want to use `fromJsonSpanned?` to set the type?
+      let a ← Json.getObjValM fObj "a"
+      let x ← Json.getObjValM a "x"
+      let exp ← Exp.fromJson x
+      return (name, exp)
+    )
+
+    match ← getDecl? pathedName with
+    | none => throw s!"[ExpX.fromJson]: Could not find datatype {pathedName}"
+    | some (Decl.struct _) => return .StructCtor dt parsedFields.toList
+    | some (Decl.enum _) => return .EnumCtor pathedName dt parsedFields.toList
+    | _ => throw s!"[ExpX.fromJson]: Encountered an unexpected decl with name {pathedName}"
+
   | ("Unary", obj) =>
     -- A unary object should be an array with an op and a data element
-    let ⟨arr, _⟩ ← coeWithState <| obj.getArrWithSizeGe? 2
-    let op   ← UnaryOp.fromJson? arr[0]
-    let data ← fromJsonSpanned? arr[1] Exp.fromJson?
+    let ⟨arr, _⟩ ← obj.getArrWithSizeGeM 2
+    let op   ← UnaryOp.fromJson arr[0]
+    let data ← fromJsonSpanned arr[1] Exp.fromJson
     return .Unary op data
+
+  | ("UnaryOpr", obj) =>
+    -- A complex unary object should be an array with an op and a data element
+    let ⟨arr, _⟩ ← obj.getArrWithSizeGeM 2
+    let op  ← UnaryOp.oprFromJson arr[0]
+    let data ← fromJsonSpanned arr[1] Exp.fromJson
+    return .Unary op data
+
   | ("Binary", obj) =>
     -- A binary object should be an array with an op and two data elements
-    let ⟨arr, _⟩ ← coeWithState <| obj.getArrWithSizeGe? 3
-    let op    ← BinaryOp.fromJson? arr[0]
-    let data₁ ← fromJsonSpanned? arr[1] Exp.fromJson?
-    let data₂ ← fromJsonSpanned? arr[2] Exp.fromJson?
+    let ⟨arr, _⟩ ← obj.getArrWithSizeGeM 3
+    let op    ← BinaryOp.fromJson arr[0]
+    let data₁ ← fromJsonSpanned arr[1] Exp.fromJson
+    let data₂ ← fromJsonSpanned arr[2] Exp.fromJson
     return .Binary op data₁ data₂
+
   | ("If", obj) =>
     -- Should be an array with three expressions
-    let ⟨arr, _⟩ ← coeWithState <| obj.getArrWithSizeGe? 3
-    let cond    ← fromJsonSpanned? arr[0] Exp.fromJson?
-    let branch₁ ← fromJsonSpanned? arr[1] Exp.fromJson?
-    let branch₂ ← fromJsonSpanned? arr[2] Exp.fromJson?
+    let ⟨arr, _⟩ ← obj.getArrWithSizeGeM 3
+    let cond    ← fromJsonSpanned arr[0] Exp.fromJson
+    let branch₁ ← fromJsonSpanned arr[1] Exp.fromJson
+    let branch₂ ← fromJsonSpanned arr[2] Exp.fromJson
     return .If cond branch₁ branch₂
+
   | ("Bind", obj) =>
     -- Should be an array with a bind and an expression
-    let ⟨arr, _⟩ ← coeWithState <| obj.getArrWithSizeGe? 2
-    let bind ← Bind.fromJson? arr[0]
-    let exp ← withBoundVars bind.idents (fromJsonSpanned? arr[1] Exp.fromJson?)
+    let ⟨arr, _⟩ ← obj.getArrWithSizeGeM 2
+    let bind ← Bind.fromJson arr[0]
+    let exp ← withBoundVars bind.idents (fromJsonSpanned arr[1] Exp.fromJson)
     return .Bind bind exp
+
   | ("Call", obj) =>
     -- Should be an object with a function name and arguments
     -- The function's name is the 0th element, the arguments the 2nd element (an array)
-    let ⟨arr, _⟩ ← coeWithState <| obj.getArrWithSizeGe? 3
-    let callFn ← CallFun.fromJson? arr[0]
-    let (expsJson : Array Json) ← arr[2].getArr?
-    let exps : Array Exp ← expsJson.mapM (fromJsonSpanned? · Exp.fromJson?)
+    let ⟨arr, _⟩ ← obj.getArrWithSizeGeM 3
+    let callFn ← CallFun.fromJson arr[0]
+    let expsJson ← arr[2].getArrM
+    let exps : Array Exp ← expsJson.mapM (fromJsonSpanned · Exp.fromJson)
     return .Call callFn [] exps.toList
+
   | s => throw s!"[ExpX.fromJson?]: Expected one of \{ Const, Var, Unary, Binary, If }, got {s}"
 
   -- | .ok ("Array", obj) =>
@@ -392,43 +471,94 @@ end /- mutual -/
 
 --------------------------------------------------------------------------------
 
-/-partial def Exp.fromFile? (path : String) : IO (Except String (Exp × VarMap)) := do
-  let jsonStr ← IO.FS.readFile path
-  let json ← IO.ofExcept <| Json.parse jsonStr
-  match Exp.fromJson? json with
-  | .ok exp (_, types) => return .ok (exp, types)
-  | .error e _ => return .error e -/
+def getSpecFnName (j : Json) : m String := do
+  let nameObj ← j.getObjValByPathM ["name"]
+  pathedNameFromJson nameObj
 
-def getSpecFnName? (j : Json) : ExStr String := do
-  let obj : Json ← j.getObjValByPath ["x", "name", "path", "segments"]
-  Json.getStr? <| ← obj.getArrVal? 0
-
-def SpecFn.fromJson? (j : Json) : ExStr SpecFn := do
+def SpecFn.fromJson (j : Json) : VParser Unit := do
   -- Parse the function name
-  let name ← getSpecFnName? j
+  let name ← getSpecFnName j
 
   -- Parse the arguments
-  let varsJson ← (← j.getObjValByPath ["x", "pars"]).getArr?
-  let vars ← varsJson.foldlM (init := Std.HashMap.empty) (fun m v => do
-    let var ← VarBinder.fromJson? (← xJsonFromSpanned? v)
-    return m.insert var.name var.val
+  let varsJson ← j.getArrUnderKeyM "pars"
+  let vars ← coeWithState <| varsJson.foldlM (init := ∅) (fun vars v => do
+    let ⟨i, ty⟩ ← VarBinder.fromJson <| ← xJsonFromSpanned v
+    return Std.HashMap.insert vars i ty
   )
 
   -- Parse the return type
-  let returnTypeJson : Json ← j.getObjValByPath ["x", "ret"]
-  let ret ← VarBinder.fromJson? (← xJsonFromSpanned? returnTypeJson)
-  let returnType : Typ := ret.val
+  let returnTypeJson : Json ← j.getObjValM "ret"
+  let ⟨_, ty⟩ ← VarBinder.fromJson <| ← xJsonFromSpanned returnTypeJson
+  let returnType : Typ := ty
 
   -- Parse the body as an expression
-  let bodyObj : Json ← j.getObjValByPath ["x", "axioms", "spec_axioms", "body_exp"]
-  match fromJsonSpanned? bodyObj Exp.fromJson? {
+  let bodyObj : Json ← j.getObjValByPath ["axioms", "spec_axioms", "body_exp"]
+  match fromJsonSpanned bodyObj Exp.fromJson {
       expectedType := returnType
       freeVars := vars
       boundVars := ∅
-      fns := Std.HashMap.empty -- CC: TODO this probably gets accumulated as we parse?
+      decls := ∅ -- CC: TODO this probably gets accumulated as we parse?
     } with
-  | .ok body _ => return SpecFn.mk name vars returnType body
   | .error e _ => throw e
+  | .ok body _ => do
+    addDecl <| SpecFn.mk name vars returnType body
+
+
+def Struct.fromJson (j : Json) : VParser Unit := do
+  let name ← pathedNameFromNameJson j "Path"
+
+  /-
+    The variants are stored in an array because Verus places structs
+    and enums into the same `DatatypeX` object. For structs, there
+    is going to be exactly one variant in the array, with its fields
+    stored in the `fields` field under the 0th entry of the outer array.
+  -/
+  let ⟨fieldsArr, _⟩ ← j.getArrUnderKeyWithSizeGeM "variants" 1
+  let fieldsArr ← fieldsArr[0].getArrUnderKeyM "fields"
+  let fields ← fieldsArr.mapM (fun f => do
+    let name ← f.getStrUnderKeyM "name"
+    let ⟨fArr, _⟩ ← f.getArrUnderKeyWithSizeGeM "a" 3
+    let typ ← Typ.fromJson fArr[0]
+    return (name, typ))
+  addDecl <| Struct.mk name [] fields.toList
+
+
+def EnumField.fromJson (j : Json) : m EnumField := do
+  let name ← j.getStrUnderKeyM "name"
+  let fieldsObj ← j.getArrUnderKeyM "fields"
+  let fields ← fieldsObj.mapM (fun f => do
+    let name ← f.getStrUnderKeyM "name"
+    -- CC: TODO for whatever reason, the type is stored in an array
+    -- CC: We default to taking the first type in this array
+    let ⟨tyArr, _⟩ ← f.getArrUnderKeyWithSizeGeM "a" 1
+    let ty ← Typ.fromJson tyArr[0]
+    return (name, ty))
+  return EnumField.mk name fields.toList
+
+
+def Enum.fromJson (j : Json) : VParser Unit := do
+  let name ← pathedNameFromNameJson j "Path"
+
+  /-
+    The variants of an enum are stored directly in the `variants` field.
+    We enforce that there should be at least one field.
+  -/
+  let ⟨fields, _⟩ ← j.getArrUnderKeyWithSizeGeM "variants" 1
+  let fields ← fields.mapM EnumField.fromJson
+  addDecl <| Enum.mk name fields.toList
+
+
+/--
+  Calls the appropriate `fromJson` helper function based on the
+  value under the `"dt_type"` key.
+-/
+def datatypeFromJson (j : Json) : VParser Unit := do
+  let dtType ← j.getStrUnderKeyM "dt_type"
+  match dtType with
+  | "Enum" => Enum.fromJson j
+  | "Struct" => Struct.fromJson j
+  | _ => throw s!"Unsupported datatype: {dtType}"
+
 
 /--
   Parses a JSON into a `Decl`, or throws an error.
@@ -444,22 +574,26 @@ def SpecFn.fromJson? (j : Json) : ExStr SpecFn := do
 partial def Decl.fromJson? (j : Json) : VParser Decl := do
   match ← j["Assert", "FuncCheckSST"] with
   | ("Assert", (obj : Json)) =>
-    -- Parse the spec functions
-    let specObjs ← coeWithState <| Json.getArr? <| ← j.getObjVal? "SpecFns"
-    let fnMap ← specObjs.foldlM (init := ∅) (fun m fnJson => do
-      let fn ← SpecFn.fromJson? fnJson
-      return Std.HashMap.insert m (SpecFn.name fn) fn
+    -- First, parse the data types (structs and enums)
+    let dtObjs ← j.getArrUnderKeyM "Datatypes"
+    let _ ← dtObjs.mapM (fun dtJson => do
+      -- Skip n-ary tuples for now (Verus places them under "Tuple")
+      -- TODO: Revisit this later (can you declare an enum named `Tuple`?)
+      match Json.getObjValByPath dtJson ["name", "Tuple"] with
+      | .ok _ => return ()
+      | .error _ => datatypeFromJson dtJson
     )
 
-    -- CC: TODO we probably shouldn't manually set the functions here (add them?)
-    setFns fnMap
+    -- Parse the spec functions
+    let specObjs ← j.getArrUnderKeyM "SpecFns"
+    let _ ← specObjs.mapM SpecFn.fromJson
 
     -- Parse the body of the assert, now that we have the spec functions
-    let exp ← Exp.fromJson? obj
+    let exp ← Exp.fromJson obj
     let vmap ← getFreeVars
 
-    let assertId ← coeWithState <| j.getNatUnderKey? "AssertId"
-    return Decl.assertion <| Assertion.mk s!"assert_{assertId}" vmap exp
+    let assertId ← j.getNatUnderKeyM "AssertId"
+    return Decl.assertion <| Assertion.mk s!"assert_{assertId}" vmap.toList exp
 
   | ("FuncCheckSST", _) => do
 
@@ -475,18 +609,10 @@ partial def Decls.fromFile? (path : String) : IO (Except String (List Decl)) := 
   let json ← IO.ofExcept <| Json.parse jsonStr
   match Decl.fromJson? json default with
   | .ok d st =>
-    let fns := st.fns.values.map (Decl.specFn ·)
-    return .ok (fns ++ [d])
+    let decls := st.decls.values
+    let dts := decls.filter (fun | .struct _ | .enum _ => true | _ => false)
+    let fns := decls.filter (fun | .specFn _ => true | _ => false)
+    return .ok (dts ++ fns ++ [d])
   | .error e _ => return .error e
-
-/-
-def FuncCheckSST.fromJson? (j : Json) : Option FuncCheckSST :=
-  -- Assume we have a top-level SST object, without a wrapping { "FuncCheckSST": ... }
-  let reqs : Exps :=
-    match j.getObjVal? "reqs" with
-    | .error _ =>
-     -/
-
-
 
 end VerusLean
